Replace Vec with Init.Data.Vector

Regex/Regex/Captures.lean
@@ -22,7 +22,7 @@ deriving Repr
 def Captures.next? (self : Captures) : Option (CapturedGroups × Captures) := do
   if self.currentPos < self.haystack.endPos then
     let buffer ← VM.captureNext self.regex.nfa self.regex.wf (self.regex.maxTag + 1) ⟨self.haystack, self.currentPos⟩
-    let groups := CapturedGroups.mk buffer.val
+    let groups := CapturedGroups.mk buffer.toArray
     let pos ← groups.get 0
     if self.currentPos < pos.2 then
       let next := { self with currentPos := pos.2 }
